\begin{align*}
  \log p(x)\\
  &= \int_z q_\phi(z|x) \log p(x) dz\\
  &= \int_z q_\phi(z|x) \log \frac{p_\theta(x,z)}{p_\theta(z|x)} dz \tag{Bayes' rule}\\
  &= \int_z q_\phi(z|x) \log\bigg(\frac{p_\theta(z,x)}{q_\phi(z|x)} \frac{q_\phi(z|x)}{p_\theta(z|x)}\bigg) dz \tag{Chain rule}\\
  &= \int_z q_\phi(z|x) \bigg(\log\frac{p_\theta(z,x)}{q_\phi(z|x)} + \log\frac{q_\phi(z|x)}{p_\theta(z|x)}\bigg) dz\\
  &= \int_z q_\phi(z|x) \log \frac{p_\theta(z,x)}{q_\phi(z|x)} dz + \int_z q_\phi(z|x) \log\frac{q_\phi(z|x)}{p_\theta(z|x)} dz\\
  &= \underbrace{\int_z q_\phi(z|x) \log \frac{p_\theta(z,x)}{q_\phi(z|x)} dz}_{= \mathcal{L}}+ \underbrace{\mathcal{D}_{\mathrm{KL}}\big(q_\phi(z|x) \| p_\theta(z|x)\big) dz}_{\geq 0}\\
  &\geq \mathcal{L}\\
\end{align*}

$\mathcal{L}$ is called the evidence lower bound with respect to $\log p(x)$.
We further rewrite $\mathcal{L}$ in order decompose the term to two separate terms, the reconstruction error $\mathcal{L}_{rec}$ and the regularizer $\mathcal{L}_{reg}$.

\begin{align*}
  \mathcal{L}
  &= \int_z q_\phi(z|x) \log\frac{p_\theta(z,x)}{q_\phi(z|x)}\\
  &= \int_z q_\phi(z|x) \log\frac{p(z) p_\theta(x|z)}{q_\phi(z|x)} \tag{we assume that x is conditionally dependent on z}\\
  &= \int_z q_\phi(z|x) \bigg(\log\frac{p(z)}{q_\phi(z|x)} + \log p_\theta(x|z)\bigg)\\
  &= -\int_z q_\phi(z|x) \log\frac{q_\phi(z|x)}{p(z)} + \int_z q_\phi(z|x) \log p_\theta(x|z)\\
  &= -\mathcal{D}_{\mathrm{KL}}\big(q_\phi(z|x) \| p(z)\big) + \int_z q_\phi(z|x) \log p_\theta(x|z)\\
  &= \underbrace{-\mathcal{D}_{\mathrm{KL}}\big(q_\phi(z|x) \| p(z)\big)}_{\mathcal{L}_{reg}} + \underbrace{\mathbb{E}_{z \sim q_\phi(z|x)}\big[ \log p_\theta(x|z)\big]}_{\mathcal{L}_{rec}}\\
  &= \mathcal{L}_{reg} + \mathcal{L}_{rec}
\end{align*}
